# 1.1 内積
### 例1.1.1
$$
\begin{aligned}
x=\begin{bmatrix} x_{1} \\ : \\ x_{n} \end{bmatrix},
y=\begin{bmatrix} y_{1} \\ : \\ y_{n} \end{bmatrix},
z =\begin{bmatrix} z_{1} \\ : \\ z_{n} \end{bmatrix}
\end{aligned}
$$

とおく。

#### (i)-1
$$
\begin{aligned}
\langle x,y+z\rangle
&=\sum ^{n}x_{i}\left( y_{i}+z_{i}\right) \\ 
&=\sum ^{n}x_{i}y_{i}+\sum ^{n}x_{i}z_{i}\\ 
&=\langle x,y\rangle +\langle x,z\rangle. 
\end{aligned}
$$

#### (i)-2
$$
\begin{aligned}
\langle x+y,z\rangle 
&=\sum ^{n}\left( x_{i}+y_{i}\right) z_{i}\\ 
&=\sum ^{n}x_{i}z_{i}+\sum ^{n}y_{i}z_{i}\\ 
&=\langle x,z\rangle +\langle y,z\rangle .
\end{aligned}
$$


#### (ii)
$$
\begin{aligned}
\langle \alpha x,y\rangle 
&=\sum ^{n}\left( \alpha x_{i}\right) y_{i}\\ 
&=\alpha \sum ^{n}x_{i}y_{i}\\ 
&=\alpha \langle x,y\rangle .
\end{aligned}
$$

同様にして、

$$
\begin{aligned}
\langle x,\alpha y\rangle 
&=\sum ^{n}x_{i}\left( \alpha y_{i}\right) \\ 
&=\alpha \sum ^{n}x_{i}y_{i}\\ 
&=\alpha \langle x,y\rangle .
\end{aligned}
$$

したがって、

$$
\langle \alpha x,y\rangle 
=\alpha \langle x,y\rangle 
=\langle x,\alpha y\rangle .
$$


#### (iii) 
$$
\begin{aligned}
\langle x,y\rangle 
&=\sum ^{n}x_{i}y_{i}\\ 
&=\sum ^{n}y_{i}x_{i}\\ 
&=\langle y,x\rangle .
\end{aligned}
$$


#### (iv)
$$
\left\| x\right\| =0
\Leftrightarrow 
x=0
$$

とおく。

$$
\Rightarrow )
$$

$$
\begin{aligned} 
\left\| x\right\| 
=\sqrt{x_{1}^{2}+\ldots +x_{n}^{2}}
=0
\end{aligned}
$$

のとき、

$$
x_{i}^2 \geq 0
$$

であるから、

$$
x_{1}^{2} = \ldots = x_{n}^{2} = 0.
$$

よって、

$$
x=
\begin{bmatrix} 
0 \\ : \\ 0 
\end{bmatrix} 
= 0.
$$

$$
\Leftarrow )
$$

$$
x=
\begin{bmatrix} 
0 \\ : \\ 0 
\end{bmatrix} 
$$

なので、

$$
\begin{aligned} 
\left\| x\right\| 
=\sqrt{0^{2}+\ldots +0^{2}}
=0.
\end{aligned}
$$

